strengthening.lean
@@ -26,16 +26,21 @@ lemma same_free_and_left {P P' Q: prop}: FV P' = FV P → (FV (P' ⋀ Q) = FV (P
     )
   )
 
+lemma free_in_left {P Q: prop}: FV P ⊆ FV (P ⋀ Q) :=
+  assume x: var,
+  assume : x ∈ FV P,
+  show x ∈ FV (P ⋀ Q), from free_in_prop.and₁ this
+
 lemma strengthen_and_with_dominating_instantiations {σ: env} {P P' Q: prop}:
-  dominates σ P P' → (σ ⊨ (P ⋀ Q).instantiated_p) → σ ⊨ (P' ⋀ Q).instantiated_p :=
-  assume h1: dominates σ P P',
+  dominates_p σ P P' → (σ ⊨ (P ⋀ Q).instantiated_p) → σ ⊨ (P' ⋀ Q).instantiated_p :=
+  assume h1: dominates_p σ P P',
   assume h2: (σ ⊨ (P ⋀ Q).instantiated_p),
-  have dominates σ (P ⋀ Q) (P' ⋀ Q), from dominates.same_right (λ_, h1),
-  dominates.elim this h2
+  have dominates_p σ (P ⋀ Q) (P' ⋀ Q), from dominates_p.same_right (λ_, h1),
+  dominates_p.elim this h2
 
 lemma strengthen_impl_with_dominating_instantiations {σ: env} {P P' Q: prop}:
-  dominates σ P' P → FV P' ⊆ FV P → (σ ⊨ (prop.implies P Q).instantiated_n) → (σ ⊨ (prop.implies P' Q).instantiated_n) :=
-  assume P'_dominates_P: dominates σ P' P,
+  dominates_p σ P' P → FV P' ⊆ FV P → (σ ⊨ (prop.implies P Q).instantiated_n) → (σ ⊨ (prop.implies P' Q).instantiated_n) :=
+  assume P'_dominates_P: dominates_p σ P' P,
   assume fv_P'_P: FV P' ⊆ FV P,
   assume h0: σ ⊨ (P.not ⋁ Q).instantiated_n,
   have h11: closed_subst σ (P'.not ⋁ Q).not.instantiated_p, from (
@@ -61,24 +66,25 @@ lemma strengthen_impl_with_dominating_instantiations {σ: env} {P P' Q: prop}:
   have (P.not ⋁ Q).not.instantiated_p = (P.not ⋁ Q).instantiated_n.not, from not_dist_instantiated_p,
   have σ ⊨ (P.not ⋁ Q).not.instantiated_p.not, from this.symm ▸ h12,
   have h2: ¬ σ ⊨ (P.not ⋁ Q).not.instantiated_p, from valid_env.not.mpr this,
+
   have h3: (σ ⊨ (P'.not ⋁ Q).not.instantiated_p) → (σ ⊨ (P.not ⋁ Q).not.instantiated_p), from (
     assume : σ ⊨ (P'.not ⋁ Q).not.instantiated_p,
     have h4: σ ⊨ (P'.not.not ⋀ Q.not).instantiated_p, from valid_env.or_not_dist_with_instantiations.mp this,
+
     have h41: σ ⊨ P'.not.not.instantiated_p, from (valid_env.and.elim (valid_env.instantiated_p_and_elim h4)).left,
     have h42: P'.not.not.instantiated_p = P'.not.instantiated_n.not, from not_dist_instantiated_p,
     have h43: P'.not.instantiated_n = P'.instantiated_p.not, from not_dist_instantiated_n,
     have σ ⊨ P'.instantiated_p.not.not, from h43 ▸ h42 ▸ h41,
     have σ ⊨ P'.instantiated_p, from valid_env.not_not.mp this,
-    have dominates σ P'.not.not P', from dominates.not_not,
-    have h5: σ ⊨ (P' ⋀ Q.not).instantiated_p,
-    from strengthen_and_with_dominating_instantiations this h4,
-    have h6: σ ⊨ (P ⋀ Q.not).instantiated_p,
-    from strengthen_and_with_dominating_instantiations P'_dominates_P h5,
-    have dominates σ P P.not.not, from dominates.of_not_not,
-    have σ ⊨ (P.not.not ⋀ Q.not).instantiated_p,
-    from strengthen_and_with_dominating_instantiations this h6,
+    have dominates_p σ P'.not.not P', from dominates_p.not_not,
+    have h5: σ ⊨ (P' ⋀ Q.not).instantiated_p, from strengthen_and_with_dominating_instantiations this h4,
+    have h6: σ ⊨ (P ⋀ Q.not).instantiated_p, from strengthen_and_with_dominating_instantiations P'_dominates_P h5,
+
+    have dominates_p σ P P.not.not, from dominates_p.of_not_not,
+    have σ ⊨ (P.not.not ⋀ Q.not).instantiated_p, from strengthen_and_with_dominating_instantiations this h6,
     show σ ⊨ (P.not ⋁ Q).not.instantiated_p, from valid_env.or_not_dist_with_instantiations.mpr this
   ),
+
   have ¬ σ ⊨ (P'.not ⋁ Q).not.instantiated_p, from mt h3 h2,
   have h9: σ ⊨ (P'.not ⋁ Q).not.instantiated_p.not, from valid_env.not.mp h11 this,
   have (P'.not ⋁ Q).not.instantiated_p = (P'.not ⋁ Q).instantiated_n.not, from not_dist_instantiated_p,
@@ -86,11 +92,11 @@ lemma strengthen_impl_with_dominating_instantiations {σ: env} {P P' Q: prop}:
   show σ ⊨ (P'.not ⋁ Q).instantiated_n, from valid_env.not_not.mp this
 
 lemma strengthen_vc {P P' Q S: prop} {σ: env}:
-  dominates σ P' P → FV P' ⊆ FV P →
+  dominates_p σ P' P → FV P' ⊆ FV P →
   (σ ⊨ (prop.implies (P ⋀ Q) S).instantiated_n) → σ ⊨ (prop.implies (P' ⋀ Q) S).instantiated_n :=
-  assume : dominates σ P' P,
+  assume : dominates_p σ P' P,
   assume fv_P'_P: FV P' ⊆ FV P,
-  have h1: dominates σ (P' ⋀ Q) (P ⋀ Q), from dominates.same_right (λ_, this),
+  have h1: dominates_p σ (P' ⋀ Q) (P ⋀ Q), from dominates_p.same_right (λ_, this),
   have h2: FV (P' ⋀ Q) ⊆ FV (P ⋀ Q), from (
     assume x: var,
     assume : x ∈ FV (P' ⋀ Q),
@@ -106,19 +112,19 @@ lemma strengthen_vc {P P' Q S: prop} {σ: env}:
   strengthen_impl_with_dominating_instantiations h1 h2
 
 lemma strengthen_exp {P: prop} {Q: propctx} {e: exp}:
-      (P ⊢ e : Q) → ∀P': prop, (FV P' = FV P) → (∀σ, dominates σ P' P) → (P' ⊢ e: Q) :=
+      (P ⊢ e : Q) → ∀P': prop, (FV P' = FV P) → (∀σ, dominates_p σ P' P) → (P' ⊢ e: Q) :=
   assume e_verified: (P ⊢ e : Q),
   begin
     induction e_verified,
     case exp.vcgen.tru x P e' Q x_not_free_in_P e'_verified ih { from (
       assume P': prop,
       assume free_P'_P: FV P' = FV P,
-      assume P'_dominates_P: (∀σ, dominates σ P' P),
+      assume P'_dominates_p_P: (∀σ, dominates_p σ P' P),
 
       have h1: FV (P' ⋀ x ≡ value.true) = FV (P ⋀ x ≡ value.true),
       from same_free_and_left free_P'_P,
-      have h2: (∀σ, dominates σ (P' ⋀ x ≡ value.true) (P ⋀ x ≡ value.true)),
-      from λσ, dominates.same_right (λ_, P'_dominates_P σ),
+      have h2: (∀σ, dominates_p σ (P' ⋀ x ≡ value.true) (P ⋀ x ≡ value.true)),
+      from λσ, dominates_p.same_right (λ_, P'_dominates_p_P σ),
       have e'_verified': P' ⋀ x ≡ value.true ⊢ e': Q, from ih (P' ⋀ x ≡ value.true) h1 h2,
       have x_not_free_in_P': x ∉ FV P', from free_P'_P.symm ▸ x_not_free_in_P,
       show P' ⊢ lett x = true in e' : propctx.exis x (x ≡ value.true ⋀ Q),
@@ -127,12 +133,12 @@ lemma strengthen_exp {P: prop} {Q: propctx} {e: exp}:
     case exp.vcgen.fals x P e' Q x_not_free_in_P e'_verified ih { from
       assume P': prop,
       assume free_P'_P: FV P' = FV P,
-      assume P'_dominates_P: (∀σ, dominates σ P' P),
+      assume P'_dominates_p_P: (∀σ, dominates_p σ P' P),
 
       have h1: FV (P' ⋀ (x ≡ value.false)) = FV (P ⋀ x ≡ value.false),
       from same_free_and_left free_P'_P,
-      have h2: (∀σ, dominates σ (P' ⋀ x ≡ value.false) (P ⋀ x ≡ value.false)),
-      from λσ, dominates.same_right (λ_, P'_dominates_P σ),
+      have h2: (∀σ, dominates_p σ (P' ⋀ x ≡ value.false) (P ⋀ x ≡ value.false)),
+      from λσ, dominates_p.same_right (λ_, P'_dominates_p_P σ),
       have e'_verified': P' ⋀ x ≡ value.false ⊢ e': Q, from ih (P' ⋀ x ≡ value.false) h1 h2,
       have x_not_free_in_P': x ∉ FV P', from free_P'_P.symm ▸ x_not_free_in_P,
       show P' ⊢ letf x = false in e' : propctx.exis x ((x ≡ value.false) ⋀ Q),
@@ -141,12 +147,12 @@ lemma strengthen_exp {P: prop} {Q: propctx} {e: exp}:
     case exp.vcgen.num x n P e' Q x_not_free_in_P e'_verified ih { from
       assume P': prop,
       assume free_P'_P: FV P' = FV P,
-      assume P'_dominates_P: (∀σ, dominates σ P' P),
+      assume P'_dominates_p_P: (∀σ, dominates_p σ P' P),
 
       have h1: FV (P' ⋀ x ≡ value.num n) = FV (P ⋀ x ≡ value.num n),
       from same_free_and_left free_P'_P,
-      have h2: (∀σ, dominates σ (P' ⋀ x ≡ value.num n) (P ⋀ x ≡ value.num n)),
-      from λσ, dominates.same_right (λ_, P'_dominates_P σ),
+      have h2: (∀σ, dominates_p σ (P' ⋀ x ≡ value.num n) (P ⋀ x ≡ value.num n)),
+      from λσ, dominates_p.same_right (λ_, P'_dominates_p_P σ),
       have e'_verified': P' ⋀ (x ≡ value.num n) ⊢ e': Q, from ih (P' ⋀ (x ≡ value.num n)) h1 h2,
       have x_not_free_in_P': x ∉ FV P', from free_P'_P.symm ▸ x_not_free_in_P,
       show P' ⊢ letn x = n in e' : propctx.exis x ((x ≡ value.num n) ⋀ Q),
@@ -156,7 +162,7 @@ lemma strengthen_exp {P: prop} {Q: propctx} {e: exp}:
                         e₁_verified e₂_verified func_vc ih₁ ih₂ { from
       assume P': prop,
       assume free_P'_P: FV P' = FV P,
-      assume P'_dominates_P: (∀σ, dominates σ P' P),
+      assume P'_dominates_p_P: (∀σ, dominates_p σ P' P),
 
       have f_not_free_in_P': f ∉ FV P', from free_P'_P.symm ▸ f_not_free_in_P,
       have x_not_free_in_P': x ∉ FV P', from free_P'_P.symm ▸ x_not_free_in_P,
@@ -165,8 +171,8 @@ lemma strengthen_exp {P: prop} {Q: propctx} {e: exp}:
 
       have h1: FV (P' ⋀ ((spec.func f x R S) ⋀ R)) = FV (P ⋀ ((spec.func f x R S) ⋀ R)),
       from same_free_and_left free_P'_P,
-      have h2: (∀σ, dominates σ (P' ⋀ (spec.func f x R S) ⋀ R) (P ⋀ (spec.func f x R S) ⋀ R)),
-      from λσ, dominates.same_right (λ_, P'_dominates_P σ),
+      have h2: (∀σ, dominates_p σ (P' ⋀ (spec.func f x R S) ⋀ R) (P ⋀ (spec.func f x R S) ⋀ R)),
+      from λσ, dominates_p.same_right (λ_, P'_dominates_p_P σ),
       have e₁_verified': P' ⋀ (spec.func f x R S) ⋀ R ⊢ e₁ : Q₁,
       from ih₁ (P' ⋀ (spec.func f x R S) ⋀ R) h1 h2,
 
@@ -174,16 +180,16 @@ lemma strengthen_exp {P: prop} {Q: propctx} {e: exp}:
              = FV (P ⋀ (prop.func f x R (Q₁ (term.app ↑f ↑x) ⋀ ↑S))),
       from same_free_and_left free_P'_P,
 
-      have h5: (∀σ, dominates σ (P' ⋀ (prop.func f x R (Q₁ (term.app ↑f ↑x) ⋀ ↑S)))
+      have h5: (∀σ, dominates_p σ (P' ⋀ (prop.func f x R (Q₁ (term.app ↑f ↑x) ⋀ ↑S)))
                       (P ⋀ (prop.func f x R (Q₁ (term.app ↑f ↑x) ⋀ ↑S)))),
-      from (λσ, dominates.same_right (λ_, P'_dominates_P σ)),
+      from (λσ, dominates_p.same_right (λ_, P'_dominates_p_P σ)),
 
       have e₂_verified': P' ⋀ (prop.func f x R (Q₁ (term.app ↑f ↑x) ⋀ ↑S)) ⊢ e₂ : Q₂,
       from ih₂ (P' ⋀ (prop.func f x R (Q₁ (term.app ↑f ↑x) ⋀ ↑S))) h3 h5,
 
       have func_vc': ∀ (σ : env),
              σ ⊨ prop.instantiated_n (prop.implies (P' ⋀ ↑(spec.func ↑f x R S) ⋀ R ⋀ Q₁ (term.app ↑f ↑x)) ↑S),
-      from (λσ, strengthen_vc (P'_dominates_P σ) (set.subset_of_eq free_P'_P) (func_vc σ)),
+      from (λσ, strengthen_vc (P'_dominates_p_P σ) (set.subset_of_eq free_P'_P) (func_vc σ)),
 
       show P' ⊢ letf f[x] req R ens S {e₁} in e₂ : propctx.exis f (prop.func f x R (Q₁ (term.app ↑f ↑x) ⋀ ↑S) ⋀ Q₂),
       from exp.vcgen.func f_not_free_in_P' x_not_free_in_P' f_neq_x x_free_in_R fv_R' fv_S' e₁_verified'
@@ -192,21 +198,21 @@ lemma strengthen_exp {P: prop} {Q: propctx} {e: exp}:
     case exp.vcgen.unop op x y P e' Q' x_free_in_P y_not_free_in_P e'_verified vc_valid ih { from
       assume P': prop,
       assume free_P'_P: FV P' = FV P,
-      assume P'_dominates_P: (∀σ, dominates σ P' P),
+      assume P'_dominates_p_P: (∀σ, dominates_p σ P' P),
 
       have x_free_in_P': x ∈ FV P', from free_P'_P.symm ▸ x_free_in_P,
       have y_not_free_in_P': y ∉ FV P', from free_P'_P.symm ▸ y_not_free_in_P,
 
       have h1: FV (P' ⋀ y ≡ term.unop op x) = FV (P ⋀ y ≡ term.unop op x),
       from same_free_and_left free_P'_P,
-      have h2: (∀σ, dominates σ (P' ⋀ y ≡ term.unop op x) (P ⋀ y ≡ term.unop op x)),
-      from (λσ, dominates.same_right (λ_, P'_dominates_P σ)),
+      have h2: (∀σ, dominates_p σ (P' ⋀ y ≡ term.unop op x) (P ⋀ y ≡ term.unop op x)),
+      from (λσ, dominates_p.same_right (λ_, P'_dominates_p_P σ)),
       have e'_verified': P' ⋀ y ≡ term.unop op x ⊢ e' : Q',
       from ih (P' ⋀ y ≡ term.unop op x) h1 h2,
 
       have FV P' ⊆ FV P, from set.subset_of_eq free_P'_P,
       have vc_valid': ∀ (σ : env), σ ⊨ prop.instantiated_n (prop.implies P' (prop.pre₁ op x)),
-      from (λσ, strengthen_impl_with_dominating_instantiations (P'_dominates_P σ) this (vc_valid σ)),
+      from (λσ, strengthen_impl_with_dominating_instantiations (P'_dominates_p_P σ) this (vc_valid σ)),
 
       show P' ⊢ letop y = op [x] in e' : propctx.exis y (y ≡ term.unop op x ⋀ Q'),
       from exp.vcgen.unop x_free_in_P' y_not_free_in_P' e'_verified' vc_valid'
@@ -214,7 +220,7 @@ lemma strengthen_exp {P: prop} {Q: propctx} {e: exp}:
     case exp.vcgen.binop op x y z e' P Q' x_free_in_P y_free_in_P z_not_free_in_P e'_verified vc_valid ih { from
       assume P': prop,
       assume free_P'_P: FV P' = FV P,
-      assume P'_dominates_P: (∀σ, dominates σ P' P),
+      assume P'_dominates_p_P: (∀σ, dominates_p σ P' P),
 
       have x_free_in_P': x ∈ FV P', from free_P'_P.symm ▸ x_free_in_P,
       have y_free_in_P': y ∈ FV P', from free_P'_P.symm ▸ y_free_in_P,
@@ -222,14 +228,14 @@ lemma strengthen_exp {P: prop} {Q: propctx} {e: exp}:
 
       have h1: FV (P' ⋀ z ≡ term.binop op x y) = FV (P ⋀ z ≡ term.binop op x y),
       from same_free_and_left free_P'_P,
-      have h2: (∀σ, dominates σ (P' ⋀ z ≡ term.binop op x y) (P ⋀ z ≡ term.binop op x y)),
-      from (λσ, dominates.same_right (λ_, P'_dominates_P σ)),
+      have h2: (∀σ, dominates_p σ (P' ⋀ z ≡ term.binop op x y) (P ⋀ z ≡ term.binop op x y)),
+      from (λσ, dominates_p.same_right (λ_, P'_dominates_p_P σ)),
       have e'_verified': P' ⋀ z ≡ term.binop op x y ⊢ e' : Q',
       from ih (P' ⋀ z ≡ term.binop op x y) h1 h2,
 
       have FV P' ⊆ FV P, from set.subset_of_eq free_P'_P,
       have vc_valid': ∀ (σ : env), σ ⊨ prop.instantiated_n (prop.implies P' (prop.pre₂ op x y)),
-      from (λσ, strengthen_impl_with_dominating_instantiations (P'_dominates_P σ) this (vc_valid σ)),
+      from (λσ, strengthen_impl_with_dominating_instantiations (P'_dominates_p_P σ) this (vc_valid σ)),
 
       show P' ⊢ letop2 z = op [x, y] in e' : propctx.exis z (z ≡ term.binop op x y ⋀ Q'),
       from exp.vcgen.binop x_free_in_P' y_free_in_P' z_not_free_in_P' e'_verified' vc_valid'
@@ -237,7 +243,7 @@ lemma strengthen_exp {P: prop} {Q: propctx} {e: exp}:
     case exp.vcgen.app y f x e' P Q' f_free_in_P x_free_in_P y_not_free_in_P e'_verified vc_valid ih { from
       assume P': prop,
       assume free_P'_P: FV P' = FV P,
-      assume P'_dominates_P: (∀σ, dominates σ P' P),
+      assume P'_dominates_p_P: (∀σ, dominates_p σ P' P),
 
       have f_free_in_P': f ∈ FV P', from free_P'_P.symm ▸ f_free_in_P,
       have x_free_in_P': x ∈ FV P', from free_P'_P.symm ▸ x_free_in_P,
@@ -247,16 +253,16 @@ lemma strengthen_exp {P: prop} {Q: propctx} {e: exp}:
              = FV (P ⋀ prop.call f x ⋀ prop.post f x ⋀ y ≡ term.app f x),
       from same_free_and_left free_P'_P,
 
-      have h2: (∀σ, dominates σ (P' ⋀ prop.call f x ⋀ prop.post f x ⋀ y ≡ term.app f x)
+      have h2: (∀σ, dominates_p σ (P' ⋀ prop.call f x ⋀ prop.post f x ⋀ y ≡ term.app f x)
                                 (P ⋀ prop.call f x ⋀ prop.post f x ⋀ y ≡ term.app f x)),
-      from (λσ, dominates.same_right (λ_, P'_dominates_P σ)),
+      from (λσ, dominates_p.same_right (λ_, P'_dominates_p_P σ)),
 
       have e'_verified': P' ⋀ prop.call f x ⋀ prop.post f x ⋀ y ≡ term.app f x ⊢ e' : Q',
       from ih (P' ⋀ prop.call f x ⋀ prop.post f x ⋀ y ≡ term.app f x) h1 h2,
 
       have vc_valid': ∀ (σ : env),
              σ ⊨ prop.instantiated_n (prop.implies (P' ⋀ prop.call f x) (term.unop unop.isFunc f ⋀ prop.pre f x)),
-      from (λσ, strengthen_vc (P'_dominates_P σ) (set.subset_of_eq free_P'_P) (vc_valid σ)),
+      from (λσ, strengthen_vc (P'_dominates_p_P σ) (set.subset_of_eq free_P'_P) (vc_valid σ)),
 
       show P' ⊢ letapp y = f [x] in e' : propctx.exis y (prop.call f x ⋀ prop.post f x ⋀ y ≡ term.app f x ⋀ Q'),
       from exp.vcgen.app f_free_in_P' x_free_in_P' y_not_free_in_P' e'_verified' vc_valid'
@@ -264,23 +270,23 @@ lemma strengthen_exp {P: prop} {Q: propctx} {e: exp}:
     case exp.vcgen.ite x e₂ e₁ P Q₁ Q₂ x_free_in_P e₁_verified e₂_verified vc_valid ih₁ ih₂ { from
       assume P': prop,
       assume free_P'_P: FV P' = FV P,
-      assume P'_dominates_P: (∀σ, dominates σ P' P),
+      assume P'_dominates_p_P: (∀σ, dominates_p σ P' P),
 
       have x_free_in_P': x ∈ FV P', from free_P'_P.symm ▸ x_free_in_P,
 
       have h1: FV (P' ⋀ x) = FV (P ⋀ x), from same_free_and_left free_P'_P,
-      have h2: (∀σ, dominates σ (P' ⋀ x) (P ⋀ x)), from (λσ, dominates.same_right (λ_, P'_dominates_P σ)),
+      have h2: (∀σ, dominates_p σ (P' ⋀ x) (P ⋀ x)), from (λσ, dominates_p.same_right (λ_, P'_dominates_p_P σ)),
       have e₁_verified': P' ⋀ x ⊢ e₁ : Q₁, from ih₁ (P' ⋀ x) h1 h2,
 
       have h1: FV (P' ⋀ term.unop unop.not x) = FV (P ⋀ term.unop unop.not x), from same_free_and_left free_P'_P,
-      have h2: (∀σ, dominates σ (P' ⋀ term.unop unop.not x) (P ⋀ term.unop unop.not x)),
-      from (λσ, dominates.same_right (λ_, P'_dominates_P σ)),
+      have h2: (∀σ, dominates_p σ (P' ⋀ term.unop unop.not x) (P ⋀ term.unop unop.not x)),
+      from (λσ, dominates_p.same_right (λ_, P'_dominates_p_P σ)),
       have e₂_verified': P' ⋀ term.unop unop.not x ⊢ e₂ : Q₂, from ih₂ (P' ⋀ term.unop unop.not x) h1 h2,
 
       have FV P' ⊆ FV P, from set.subset_of_eq free_P'_P,
       have vc_valid': ∀ (σ : env),
              σ ⊨ prop.instantiated_n (prop.implies P' (term.unop unop.isBool x)),
-      from (λσ, strengthen_impl_with_dominating_instantiations (P'_dominates_P σ) this (vc_valid σ)),
+      from (λσ, strengthen_impl_with_dominating_instantiations (P'_dominates_p_P σ) this (vc_valid σ)),
 
       show P' ⊢ exp.ite x e₁ e₂ : propctx.implies x Q₁ ⋀ propctx.implies (term.unop unop.not x) Q₂,
       from exp.vcgen.ite x_free_in_P' e₁_verified' e₂_verified' vc_valid'
@@ -288,7 +294,7 @@ lemma strengthen_exp {P: prop} {Q: propctx} {e: exp}:
     case exp.vcgen.return x P x_free_in_P { from
       assume P': prop,
       assume free_P'_P: FV P' = FV P,
-      assume P'_dominates_P: (∀σ, dominates σ P' P),
+      assume P'_dominates_p_P: (∀σ, dominates_p σ P' P),
 
       have x_free_in_P': x ∈ FV P', from free_P'_P.symm ▸ x_free_in_P,
 
